fix bug in function symbolsToExchange, prove lemma_Exchange_Generates_One_SymbolSeq_For_Each_Node

bce/service.dfy
@@ -18,6 +18,7 @@ datatype Service = Service(
 /****************************************************************************************/   
 
 
+/* True iff Service state s is a valid initial state */
 predicate serviceInit(s: Service)
 {
     && s.f > 0
@@ -31,11 +32,12 @@ predicate serviceExchangeSymbols(s: Service, s': Service)
     requires serviceInit(s)
 {
     var symbolsForExchange := symbolsToExchange(s.nodes);
-    lemma_Exchange_Generates_One_SymbolSeq_For_Each_Node(s.nodes);
-    lemma_Extract_Generates_One_Symbol_For_Each_Node(s.nodes);
+    // symbolsForExchange[i] is the seq of symbols that node i receives.
+    // For any node i, symbolsForExchange[i][j] contains the jth symbol of node j.
     lemma_Exchanged_Symbols_Are_Extracted(s.nodes, symbolsForExchange, 0);
     assert |symbolsForExchange| == |s.nodes|;
-    && s' == s.(nodes := s'.nodes)
+    assert forall sym :: sym in symbolsForExchange ==> |sym| == |s.nodes|;
+    && s' == s.(nodes := s'.nodes, state := SPhase2)
     && |s'.nodes| == |s.nodes|
     && forall id :: 0 <= id < |s.nodes| ==> 
         assert symbolsForExchange[id][id] == s.nodes[id].codeword[id];
@@ -59,13 +61,23 @@ predicate serviceNext(s:Service, s':Service)
 * symbolsToExchange(nodes)[i] represents the seq of symbols that nodes[i] receives in 
 * the exhange phase */
 function symbolsToExchange(nodes: seq<Node>) : seq<seq<symbol>> 
-    decreases nodes;
     requires forall s :: s in nodes ==> s.n == 3*s.f + 1;
     requires forall s :: s in nodes ==> 0 <= s.id < s.n;
     requires forall s :: s in nodes ==> nodeInit(s, s.f, s.n, s.id)
 {
-    if |nodes| == 0 then [] else
-    [extractSymbols(nodes)] + symbolsToExchange(nodes[1..])
+    symbolsToExchangeHelper(nodes, 0)
+}
+
+
+function symbolsToExchangeHelper(nodes: seq<Node>, i: nat) : seq<seq<symbol>> 
+    decreases |nodes| - i;
+    requires 0 <= i <= |nodes|;
+    requires forall s :: s in nodes ==> s.n == 3*s.f + 1;
+    requires forall s :: s in nodes ==> 0 <= s.id < s.n;
+    requires forall s :: s in nodes ==> nodeInit(s, s.f, s.n, s.id)
+{
+    if i == |nodes| then [] else
+    [extractSymbols(nodes)] + symbolsToExchangeHelper(nodes, i + 1)
 }
 
 /* Helper function that generates a single seq<symbol> for exchange. 
@@ -87,12 +99,21 @@ function extractSymbols(nodes: seq<Node>) : seq<symbol>
 
 
 /* Proof that for any nodes: seq<Node>, |symbolsToExchange(nodes)| == |nodes| */
-lemma {:induction nodes} lemma_Exchange_Generates_One_SymbolSeq_For_Each_Node(nodes: seq<Node>) 
+lemma {:induction i} lemma_Exchange_Generates_One_SymbolSeq_For_Each_Node(nodes: seq<Node>, i:nat) 
+    decreases |nodes| - i;
+    requires 0 <= i <= |nodes|;
     requires forall s :: s in nodes ==> s.n == 3*s.f + 1;
     requires forall s :: s in nodes ==> 0 <= s.id < s.n;
     requires forall s :: s in nodes ==> nodeInit(s, s.f, s.n, s.id)
-    ensures |symbolsToExchange(nodes)| == |nodes|;
-{}
+    requires symbolsToExchangeHelper(nodes, 0) == symbolsToExchange(nodes);
+    ensures |symbolsToExchangeHelper(nodes, i)| == |nodes[i..]|;
+{
+    if i == |nodes| {
+        assert |symbolsToExchangeHelper(nodes, i)| == 0;
+    } else {
+        lemma_Exchange_Generates_One_SymbolSeq_For_Each_Node(nodes, i+1);
+    }
+}
 
 
 /* Proof that for any nodes: seq<Node>, |extractSymbols(nodes)| == |nodes| */
@@ -107,10 +128,18 @@ lemma {:induction nodes} lemma_Extract_Generates_One_Symbol_For_Each_Node(nodes:
 lemma  {:induction nodes} lemma_Exchanged_Symbols_Are_Extracted(nodes: seq<Node>, symbolsForExchange: seq<seq<symbol>>, i: nat) 
     requires forall s :: s in nodes ==> s.n == 3*s.f + 1;
     requires forall s :: s in nodes ==> 0 <= s.id < s.n;
-    requires forall s :: s in nodes ==> nodeInit(s, s.f, s.n, s.id)
+    requires forall s :: s in nodes ==> nodeInit(s, s.f, s.n, s.id);
+    requires symbolsForExchange == symbolsToExchange(nodes);
+    ensures |symbolsForExchange| == |nodes|;
+    ensures |extractSymbols(nodes)| == |nodes|;
     ensures forall id :: 0 <= id < |symbolsForExchange| ==> symbolsForExchange[id] == extractSymbols(nodes);
 {
     //TODO
+    lemma_Extract_Generates_One_Symbol_For_Each_Node(nodes);
+    lemma_Exchange_Generates_One_SymbolSeq_For_Each_Node(nodes, 0);
+    assert |symbolsForExchange| == |nodes|;
+    assert forall id :: 0 <= id < |symbolsForExchange| ==> symbolsForExchange[id] == extractSymbols(nodes);
+    // assert forall symbseq :: symbseq in symbolsForExchange ==> symbseq == extractSymbols(nodes);
 }
 
 
